ProofWidgets/Demos/ContourInteractive.lean
@@ -8,10 +8,12 @@ structure point where
   y : Float
   deriving ToJson, FromJson
 structure line where
+  label : String
   startPoint : point
   endPoint : point
   deriving ToJson, FromJson
 structure arc where
+  labe : String
   center : point
   radius : Float
   startAngle : Float
@@ -24,11 +26,13 @@ structure ContourProps where
   nodes : Array point := #[]
   edges : Array line := #[]
   arcs : Array arc := #[]
+  selectedLabels : Option (Array String) := none
     deriving ToJson, FromJson, Inhabited
 
 @[widget_module]
 def Contour : Component ContourProps where
   javascript := include_str ".." / ".." / "build" / "js" / "contour.js"
 
-#html <Contour nodes = {#[⟨20, 20⟩, ⟨4.5, 6.0⟩]} edges = {#[⟨⟨10, 10⟩, ⟨500, 10⟩⟩]} arcs = {#[⟨⟨500, 10⟩, 10, 0, 3.14 * 2⟩, ⟨⟨500 - 20, 10⟩, 20, 0, 3.14⟩]} />
-#eval ToJson.toJson ({nodes := #[⟨3.0, 5.0⟩, ⟨4.5, 6.0⟩], edges := #[⟨⟨1.0, 2.0⟩, ⟨50, 50⟩⟩], arcs := #[]} : ContourProps)
+#html <Contour nodes = {#[⟨20, 20⟩, ⟨4.5, 6.0⟩]} edges = {#[⟨"klj", ⟨10, 10⟩, ⟨500, 10⟩⟩, ⟨"kl", ⟨10, 10⟩, ⟨10, 500⟩⟩]} arcs = {#[⟨"l", ⟨500, 10⟩, 10, 0, 3.14 * 2⟩, ⟨"h7", ⟨500 - 20, 10⟩, 40, 0, 3.14⟩]} selectedLabels={#["klj"]}/>
+#eval ToJson.toJson ({nodes := #[⟨20, 20⟩, ⟨4.5, 6.0⟩], edges := #[⟨"", ⟨10, 10⟩, ⟨500, 10⟩⟩], arcs := #[⟨"lkj", ⟨500, 10⟩, 10, 0, 3.14 * 2⟩, ⟨"h7", ⟨500 - 20, 10⟩, 20, 0, 3.14⟩]} : ContourProps)
+-- #eval ToJson.toJson ({nodes := #[⟨3.0, 5.0⟩, ⟨4.5, 6.0⟩], edges := #[⟨⟨1.0, 2.0⟩, ⟨50, 50⟩⟩], arcs := #[]} : ContourProps)
